stlc/soundness.v
@@ -11,18 +11,22 @@ Proof.
   intros e1 t H1.
   remember cempty as c eqn:H in H1.
   induction H1 as [
-    c                           |
-    c x t H1                    |
-    c x e t1 t2 H1 IH           |
-    c e1 e2 t1 t2 H1 IH1 H2 IH2
+    c                           (* tUnit *)
+  | c x t H1                    (* tVar  *)
+  | c x e t1 t2 H1 IH           (* tAbs  *)
+  | c e1 e2 t1 t2 H1 IH1 H2 IH2 (* tApp  *)
   ].
+  (* tUnit *)
   - right.
     apply valUnit.
+  (* tVar *)
   - rewrite H in H1.
     simpl in H1.
     discriminate H1.
+  (* tAbs *)
   - right.
     apply valAbs.
+  (* tApp *)
   - left.
     elim (IH1 H).
     + intros H3.
@@ -41,7 +45,9 @@ Proof.
       * {
         intros H4.
         destruct H3.
+        (* eunit *)
         - inversion H1.
+        (* eabs x t e *)
         - exists (subst e0 x e1).
           apply stAppAbs.
           assumption.
@@ -52,7 +58,7 @@ Lemma contextInvariance :
   forall c1 c2 e t1,
   hasType c1 e t1 -> (
     forall x,
-    varIsFreeInTerm x e = true ->
+    freeVar x e ->
     lookupEvar c1 x = lookupEvar c2 x
   ) ->
   hasType c2 e t1.
@@ -61,107 +67,105 @@ Proof.
   generalize c2.
   clear c2.
   induction H1 as [
-    c1                            |
-    c1 x1 t1 H1                   |
-    c1 x1 e1 t1 t2 H1 IH          |
-    c1 e1 e2 t1 t2 H1 IH1 H2 IH2
+    c1                           (* tUnit *)
+  | c1 x1 t1 H1                  (* tVar  *)
+  | c1 x1 e1 t1 t2 H1 IH         (* tAbs  *)
+  | c1 e1 e2 t1 t2 H1 IH1 H2 IH2 (* tApp  *)
   ].
+  (* tUnit *)
   - intros.
     apply tUnit.
+  (* tVar *)
   - intros c2 H2.
     apply tVar.
     rewrite <-H1.
     symmetry.
     apply H2.
-    simpl.
-    destruct (eqId idTerm x1 x1); congruence.
+    apply freeEvar.
+    reflexivity.
+  (* tAbs *)
   - intros c2 H2.
     apply tAbs.
     apply IH.
     simpl.
     intros x2 H3.
-    destruct (eqId idTerm x2 x1) eqn:H4.
-    + congruence.
+    destruct (eqId idTerm x2 x1) as [ H4 | H4 ].
+    (* eqId idTerm x2 x1 = left e *)
+    + reflexivity.
+    (* eqId idTerm x2 x1 = right n *)
     + apply H2.
-      simpl.
-      rewrite H4.
-      congruence.
+      apply freeAbs; assumption.
+  (* tApp *)
   - intros c2 H3.
     apply tApp with (t1 := t1).
+    (* hastype c2 e2 (tarrow t1 t2) *)
     + apply IH1.
       intros x1 H4.
       apply H3.
-      simpl.
-      apply orb_true_iff.
-      left.
+      apply freeApp2.
       assumption.
+    (* hasType c2 e1 t1 *)
     + apply IH2.
       intros x1 H4.
       apply H3.
-      simpl.
-      apply orb_true_iff.
-      right.
+      apply freeApp1.
       assumption.
 Qed.
 
 Lemma freeVarsAppearInContext :
   forall c e x t1,
   hasType c e t1 ->
-  varIsFreeInTerm x e = true ->
+  freeVar x e ->
   exists t2,
   lookupEvar c x = Some t2.
 Proof.
-  intros c1 e1 x1.
-  generalize c1.
-  clear c1.
-  induction e1 as [
-                 |
-    x2           |
-    x2 t2 e1 IH  |
-    e1 IH1 e2 IH2
+  intros c1 e1 x1 t1 H1 H2.
+  induction H1 as [
+    c1                           (* tUnit *)
+  | c1 x2 t1 H1                  (* tVar  *)
+  | c1 x2 e1 t1 t2 H1 IH         (* tAbs  *)
+  | c1 e1 e2 t1 t2 H1 IH1 H3 IH2 (* tApp  *)
   ].
-  - intros c1 t1 H1 H2.
-    inversion H2.
-  - intros c1 t1 H1 H2.
-    inversion H1 as [
-                            |
-      c2 x3 t2 H3 H4 H5 H6  |
-                            |
-
+    (* tUnit *)
+  - inversion H2.
+    (* tVar *)
+  - exists t1.
+    inversion H2 as [
+      x3 H3 H4 (* freeEvar *)
+    |          (* freeAbs  *)
+    |          (* freeApp1 *)
+    |          (* freeApp2 *)
     ].
-    simpl in H2.
-    destruct (eqId idTerm x1 x2).
-    + exists t1.
-      congruence.
-    + inversion H2.
-  - intros c1 t1 H1 H2.
-    inversion H1 as [
-                                  |
-                                  |
-      c2 x3 e2 t3 t4 H3 H4 H5 H6  |
+    congruence.
+    (* tAbs *)
+  - inversion H2 as [
+                        (* freeEvar *)
+    | x4 t3 e2 H3 H4 H5 (* freeAbs  *)
+    |                   (* freeApp1 *)
+    |                   (* freeApp2 *)
     ].
-    set (H7 := IH (cextend c1 x2 t2) t3 H3).
-    simpl in H2.
-    destruct (eqId idTerm x1 x2) eqn:H8.
-    + inversion H2.
-    + apply H7 in H2.
-      destruct H2 as [ t5 ].
-      simpl in H2.
-      rewrite H8 in H2.
-      exists t5.
+    apply IH in H4.
+    destruct H4 as [ t4 ].
+    exists t4.
+    simpl in H4.
+    destruct (eqId idTerm x1 x2) as [ Eq | Neq ].
+    (* x1 = x2 *)
+    + contradiction.
+    (* x1 <> x2 *)
+    + assumption.
+    (* tApp *)
+  - inversion H2 as [
+                        (* freeEvar *)
+    |                   (* freeAbs  *)
+    | e3 e4 H4 H5       (* freeApp1 *)
+    | e3 e4 H4 H5       (* freeApp2 *)
+    ].
+    (* freeApp1 *)
+    + apply IH2.
       assumption.
-  - intros c1 t1 H1 H2.
-    simpl in H2.
-    inversion H1 as [
-                                    |
-                                    |
-                                    |
-      c2 e3 e4 t2 t3 H3 H4 H5 H6 H7
-    ].
-    apply orb_true_iff in H2.
-    destruct H2.
-    + apply IH1 with (t1 := (tarrow t2 t1)); assumption.
-    + apply IH2 with (t1 := t2); assumption.
+    (* freeApp2 *)
+    + apply IH1.
+      assumption.
 Qed.
 
 Lemma swapVarsInContext :
@@ -172,11 +176,15 @@ Lemma swapVarsInContext :
 Proof.
   intros c1 x1 x2 x3 t1 t2 H1.
   simpl.
-  destruct (eqId idTerm x3 x2).
-  - destruct (eqId idTerm x3 x1).
-    + rewrite e0 in e.
+  destruct (eqId idTerm x3 x2) as [ Eq1 | Neq1 ].
+  (* x3 = x2 *)
+  - destruct (eqId idTerm x3 x1) as [ Eq2 | Neq2 ].
+    (* x3 = x1 *)
+    + rewrite Eq2 in Eq1.
       contradiction.
+    (* x3 <> x1 *)
     + reflexivity.
+  (* x3 <> x2 *)
   - destruct (eqId idTerm x3 x1); reflexivity.
 Qed.
 
@@ -190,48 +198,70 @@ Proof.
   generalize c1.
   clear c1.
   induction e1 as [
-                      |
-    x2                |
-    x2 t3 e1 IH       |
-    e1 IH1 e3 IH2
+                  (* eunit *)
+  | x2            (* evar  *)
+  | x2 t3 e1 IH   (* eabs  *)
+  | e1 IH1 e3 IH2 (* eapp  *)
   ].
+  (* eunit *)
   - simpl.
     intros c1 t1 t2 H1 H2.
     inversion H1.
     apply tUnit.
+  (* evar *)
   - intros c1 t1 t2 H1 H2.
     simpl.
     destruct (eqId idTerm x1 x2) eqn:H3.
+    (* x1 = x2 *)
     + rewrite e in H1.
-      inversion H1.
+      inversion H1 as [
+                    (* tUnit *)
+      | c2 x3 t3 H4 (* tVar  *)
+      |             (* tAbs  *)
+      |             (* tApp  *)
+      ].
       apply contextInvariance with (c1 := cempty).
+      (* hasType cempty e2 t1 *)
       * simpl in H4.
         rewrite e in H3.
         rewrite H3 in H4.
         congruence.
+      (* free variables occur in both contexts *)
       * {
-        intros x3 H6.
+        intros x4 H6.
         apply freeVarsAppearInContext with (c := cempty) (t1 := t2) in H6.
+        (* lookupEvar cempty x4 = lookupEvar c1 x4 *)
         - destruct H6.
           inversion H6.
+        (* hasType cempty e2 t2 *)
         - assumption.
         }
+    (* hasType c1 (evar x2) t1 *)
     + apply tVar.
-      inversion H1.
+      inversion H1 as [
+                             (* tUnit *)
+      | c2 x3 t3 H4 H5 H6 H7 (* tVar  *)
+      |                      (* tAbs  *)
+      |                      (* tApp  *)
+      ].
       simpl in H4.
-      destruct (eqId idTerm x2 x1).
+      destruct (eqId idTerm x2 x1) as [ Eq | Neq ].
+      (* x1 = x2 *)
       * contradiction n.
         congruence.
+      (* x1 <> x2 *)
       * assumption.
+  (* eabs *)
   - intros c1 t1 t2 H1 H2.
     simpl.
     inversion H1 as [
-                                 |
-                                 |
-      c2 x3 e3 t4 t5 H4 H5 H6 H7 |
-
+                                 (* tUnit *)
+    |                            (* tVar  *)
+    | c2 x3 e3 t4 t5 H4 H5 H6 H7 (* tAbs  *)
+    |                            (* tApp  *)
     ].
     destruct (eqId idTerm x1 x2) eqn:H8.
+    (* x1 = x2 *)
     + apply tAbs.
       rewrite e in H4.
       apply contextInvariance with (c1 := cextend (cextend c1 x2 t2) x2 t3).
@@ -239,8 +269,10 @@ Proof.
       * intros x4 H9.
         simpl.
         destruct (eqId idTerm x4 x2); congruence.
+    (* x1 <> x2 *)
     + apply tAbs.
       apply IH with (t2 := t2).
+      (* hasType (cextend (cextend c1 x2 t3) x1 t2) e1 t4 *)
       * {
         apply contextInvariance with (c1 := cextend (cextend c1 x1 t2) x2 t3).
         - congruence.
@@ -248,18 +280,21 @@ Proof.
           apply swapVarsInContext.
           assumption.
         }
-      * simpl.
-        assumption.
+      (* hasType cempty e2 t2 *)
+      * assumption.
+  (* eapp *)
   - intros c1 t1 t2 H1 H2.
     simpl.
     inversion H1 as [
-                                    |
-                                    |
-                                    |
-      c2 e4 e5 t3 t4 H4 H5 H6 H7 H8
+                                    (* tUnit *)
+    |                               (* tVar  *)
+    |                               (* tAbs  *)
+    | c2 e4 e5 t3 t4 H4 H5 H6 H7 H8 (* tApp  *)
     ].
     apply tApp with (t1 := t3).
+    (* hasType c1 (subst e1 x1 e2) (tarrow t3 t1) *)
     + apply IH1 with (t2 := t2); assumption.
+    (* hasType c1 (subst e3 x1 e2) t3 *)
     + apply IH2 with (t2 := t2); assumption.
 Qed.
 
@@ -274,33 +309,42 @@ Proof.
   clear e2.
   remember cempty as c eqn:H2 in H1.
   induction H1 as [
-                                |
-    c x t H1                    |
-    c x e t1 t2 H1 IH           |
-    c e1 e3 t1 t2 H1 IH1 H3 IH2
+                                (* tUnit *)
+  | c x t H1                    (* tVar  *)
+  | c x e t1 t2 H1 IH           (* tAbs  *)
+  | c e1 e3 t1 t2 H1 IH1 H3 IH2 (* tApp  *)
   ].
-  - intros e2 H.
-    inversion H.
-  - intros e2 H.
-    inversion H.
-  - intros e2 H.
-    inversion H.
+  (* tUnit *)
+  - intros e2 H1.
+    inversion H1.
+  (* tVar *)
+  - intros e2 H3.
+    inversion H3.
+  (* tAbs *)
+  - intros e2 H3.
+    inversion H3.
+  (* tApp *)
   - intros e2 H4.
     inversion H4 as [
-      x e4 e5 t3 H5 H6 H7  |
-      e4 e5 e6 H5 H6 H7    |
-      e4 e5 e6 H5 H6 H7 H8
+      x e4 e5 t3 H5 H6 H7  (* stAppAbs *)
+    | e4 e5 e6 H5 H6 H7    (* stApp1   *)
+    | e4 e5 e6 H5 H6 H7 H8 (* stApp2   *)
     ].
+    (* stAppAbs *)
     + clear IH1 IH2.
       apply substPreservesType with (t2 := t1).
+      (* hasType (cextend cempty x t1) e4 t2 *)
       * rewrite <-H6 in H1.
         inversion H1.
         congruence.
+      (* hasType cempty e1 t1 *)
       * congruence.
+    (* stApp1 *)
     + set (H8 := IH1 H2 e5 H5).
       rewrite H2 in H3.
       set (H9 := tApp cempty e1 e5 t1 t2 H8 H3).
       assumption.
+    (* stApp2 *)
     + set (H9 := IH2 H2 e6 H6).
       rewrite H2 in H1.
       set (H10 := tApp cempty e6 e3 t1 t2 H1 H9).
